Add current result of SIMT_verification_util.v.

SIMT_verification_util.v
@@ -6,28 +6,44 @@ Section SIMT_verification_util.
   Variable num_threads : {n : nat | 0 < n}.
   Definition N := sval num_threads.
 
-
   Inductive program_with_inv : Type :=
-  | Prg : program -> program_with_inv
+  | asgn' : forall n, V n -> n.-tuple E -> E -> program_with_inv
+  | skip' : program_with_inv
+  | sync' : program_with_inv
   | seq' : program_with_inv -> program_with_inv -> program_with_inv
   | P_if' : E -> program_with_inv -> program_with_inv -> program_with_inv
   | P_while' : E -> program_with_inv -> assertion num_threads -> program_with_inv.
   Notation "'WHILE' e 'DO' P 'with' phi" := (P_while' e P phi) (at level 140).
   Notation "s '[[' e ']](' i ')'" := (E_under_state num_threads s e i) (at level 50).
+(*
+  Fixpoint emb_with_inv (P : program) : program_with_inv :=
+    match P with
+    | asgn n v es e => asgn' n v es e
+    | skip => skip'
+    | sync => sync'
+    | seq P Q => seq' (emb_with_inv P) (emb_with_inv Q)
+    | P_if e P Q => P_if' e (emb_with_inv P) (emb_with_inv Q)
+    | P_while' 
   Coercion Prg : program >-> program_with_inv.
-
+ *)
   Fixpoint remove_inv (P : program_with_inv) : program :=
     match P with
-      | Prg p => p
-      | seq' p p' => SIMT.seq (remove_inv p) (remove_inv p')
-      | P_if' e p p' => P_if e (remove_inv p) (remove_inv p')
-      | P_while' e p _ => P_while e (remove_inv p)
+    | asgn' n v es e => asgn n v es e
+    | skip' => skip
+    | sync' => sync
+    | seq' p p' => SIMT.seq (remove_inv p) (remove_inv p')
+    | P_if' e p p' => P_if e (remove_inv p) (remove_inv p')
+    | P_while' e p _ => P_while e (remove_inv p)
     end.
 
-
   Inductive Hoare_proof' : assertion num_threads -> (T num_threads -> int) -> program_with_inv -> assertion num_threads -> Prop :=
-  | hoare_pf : forall phi m (P : program) psi, Hoare_proof _ phi m P psi ->
-                                               Hoare_proof' phi m P psi
+  | H_Skip' : forall phi m, Hoare_proof' phi m skip' phi
+  | H_Sync' : forall (phi : assertion num_threads) m, Hoare_proof' (fun s => (all num_threads m \/ none num_threads m) -> phi s) m sync' phi
+  | H_Assign' : forall n x es e m (phi : assertion num_threads),
+      Hoare_proof' (fun s : state num_threads =>
+                      forall x', assign num_threads s n x' m x es e ->
+                                 phi (update_state num_threads s n x x'))
+                   m (asgn' n x es e) phi
   | H_Conseq' : forall (phi phi' psi psi' : assertion _) m P,
                   Hoare_proof' phi m P psi ->
                   (forall s, phi' s -> phi s) ->
@@ -46,12 +62,32 @@ Section SIMT_verification_util.
                  Hoare_proof' phi m (WHILE e DO P with phi) (fun s => phi s /\ none _ (fun i : T _ => e_and [tuple m i; s[[e]](i)])).
 
 
+
+  Lemma H_Conseq_pre' : forall (phi psi phi' : assertion num_threads) m p,
+                         Hoare_proof' phi' m p psi ->
+                         (forall s, phi s -> phi' s) ->
+                         Hoare_proof' phi m p psi.
+  Proof.
+    intros.
+    apply (H_Conseq' _ _ _ _ m p H H0 (fun s => id)).
+  Qed.
+
+  Lemma H_Conseq_post' : forall (phi psi psi' : assertion num_threads) m p,
+                         Hoare_proof' phi m p psi' ->
+                         (forall s, psi' s -> psi s) ->
+                         Hoare_proof' phi m p psi.
+  Proof.
+    intros.
+    apply (H_Conseq' _ _ _ _ m p H (fun s => id) H0).
+  Qed.
+
   Lemma hoare_proof_remove_inv : forall phi m P psi,
                                    Hoare_proof' phi m P psi ->
                                    Hoare_proof _ phi m (remove_inv P) psi.
   Proof.
     move=> phi m P psi H.
-    induction H => //= .
+    induction H => //= ; try (econstructor; fail).
+    { eapply H_Assign; eassumption. }
     { eapply H_Conseq; eassumption. }
     { eapply H_Seq; eassumption. }
     { eapply H_If; eassumption. }
